intermediate/Veritas.Intermediate.TSLog.fsti
@@ -102,7 +102,7 @@ val lemma_to_logk_thread_count (#vcfg:_) (il:its_log vcfg)
 
 val lemma_to_logk_thread_id_of (#vcfg:_) (il:its_log vcfg) (i:I.seq_index il)
   : Lemma (ensures thread_id_of il i == SpecTS.thread_id_of (to_logk il) i)
-          [SMTPat (SpecTS.thread_id_of (to_logk il) i)]
+          [SMTPat (thread_id_of il i)]
 
 val lemma_to_logk_prefix_commute (#vcfg:_) (il:its_log vcfg) (i:nat{i <= I.length il})
   : Lemma (to_logk (I.prefix il i) == I.prefix (to_logk il) i)
